making the rewriter a bit more rohbust.

theories/RTac/SolveK.v
@@ -1,5 +1,5 @@
 Require Import ExtLib.Tactics.
-Require Import MirrorCore.RTac.Core.
+Require Import MirrorCore.RTac.CoreK.
 Require Import MirrorCore.RTac.IsSolved.
 
 Require Import MirrorCore.Util.Forwardy.
@@ -15,17 +15,17 @@ Section parameterized.
   Context {Typ0_Prop : Typ0 _ Prop}.
   Context {ExprUVar_expr : ExprUVar expr}.
 
-  Definition SOLVE (tac : rtac typ expr) : rtac typ expr :=
+  Definition SOLVEK (tac : rtacK typ expr) : rtacK typ expr :=
     fun tus tvs nus nvs ctx s g =>
       match is_solved (tac tus tvs nus nvs ctx s g) with
       | Some s => Solved s
       | _ => Fail
       end.
 
-  Theorem SOLVE_sound
-  : forall tac, rtac_sound tac -> rtac_sound (SOLVE tac).
+  Theorem SOLVEK_sound
+  : forall tac, rtacK_sound tac -> rtacK_sound (SOLVEK tac).
   Proof.
-    unfold SOLVE, rtac_sound.
+    unfold SOLVEK, rtacK_sound.
     intros.
     specialize (H ctx s g).
     destruct (is_solved (tac (getUVars ctx) (getVars ctx) (length (getUVars ctx))
@@ -37,11 +37,22 @@ Section parameterized.
     { eapply H. reflexivity. }
   Qed.
 
-  Fixpoint SOLVES (tacs : list (rtac typ expr)) : rtac typ expr :=
+  Theorem WF_SOLVEK : forall tac, WellFormed_rtacK tac -> WellFormed_rtacK (SOLVEK tac).
+  Proof.
+    unfold SOLVEK, WellFormed_rtacK. intros.
+    subst. unfold rtacK_spec_wf in *.
+    specialize (H ctx s g _ eq_refl).
+    destruct (tac (getUVars ctx) (getVars ctx) (length (getUVars ctx))
+                  (length (getVars ctx)) ctx s g); simpl; auto.
+    destruct (is_solved_goal g0); auto.
+    tauto.
+  Qed.
+
+  Fixpoint SOLVESK (tacs : list (rtacK typ expr)) : rtacK typ expr :=
     match tacs with
     | nil => fun tus tvs nus nvs ctx s g => Fail
     | tac :: tacs =>
-      let rec := SOLVES tacs in
+      let rec := SOLVESK tacs in
       fun tus tvs nus nvs ctx s g =>
         match is_solved (tac tus tvs nus nvs ctx s g) with
         | Some s => Solved s
@@ -50,7 +61,7 @@ Section parameterized.
     end.
 
   Theorem SOLVES_sound
-  : forall tacs, Forall rtac_sound tacs -> rtac_sound (SOLVES tacs).
+  : forall tacs, Forall rtacK_sound tacs -> rtacK_sound (SOLVESK tacs).
   Proof.
     induction 1; simpl.
     { red. intros; subst. eapply rtac_spec_Fail. }
@@ -67,5 +78,5 @@ Section parameterized.
 
 End parameterized.
 
-Arguments SOLVE {_ _} _%rtac _ _ _ _ _ _ _.
-Arguments SOLVES {_ _} _%or_rtac _ _ _ _ _ _ _.
+Arguments SOLVEK {_ _} _%rtac _ _ _ _ _ _ _.
+Arguments SOLVESK {_ _} _%or_rtac _ _ _ _ _ _ _.
